fr.inria.atlanmod.coqtl.coq/core/modeling/ModelingSemantics.v
@@ -54,27 +54,27 @@ Section SemanticsModeling.
   Definition resolveIter (tls: list TraceLink) (sm: SourceModel) (name: string)
              (type: TargetModelClass) (sp: list SourceModelElement)
              (iter : nat) : option (denoteModelClass type) :=
-    denoteOutput type (resolveIter' tls sm name sp iter).
+    denoteOutput type (resolveIter tls sm name sp iter).
 
   Definition resolve (tr: list TraceLink) (sm: SourceModel) (name: string)
     (type: TargetModelClass) (sp: list SourceModelElement) : option (denoteModelClass type) :=
-    denoteOutput type (resolve' tr sm name sp).
+    denoteOutput type (resolve tr sm name sp).
 
   Definition resolveAllIter (tr: list TraceLink) (sm: SourceModel) (name: string)
     (type: TargetModelClass) (sps: list(list SourceModelElement)) (iter: nat)
     : option (list (denoteModelClass type)) :=
-    denoteOutputList type (resolveAllIter' tr sm name sps iter).
+    denoteOutputList type (resolveAllIter tr sm name sps iter).
 
   Definition resolveAll (tr: list TraceLink) (sm: SourceModel) (name: string)
     (type: TargetModelClass) (sps: list(list SourceModelElement)) : option (list (denoteModelClass type)) :=
-    denoteOutputList type (resolveAll' tr sm name sps).
+    denoteOutputList type (resolveAll tr sm name sps).
   
   Definition maybeResolve (tr: list TraceLink) (sm: SourceModel) (name: string)
     (type: TargetModelClass) (sp: option (list SourceModelElement)) : option (denoteModelClass type) :=
-    denoteOutput type (maybeResolve' tr sm name sp).
+    denoteOutput type (maybeResolve tr sm name sp).
 
   Definition maybeResolveAll (tr: list TraceLink) (sm: SourceModel) (name: string)
     (type: TargetModelClass) (sp: option (list (list SourceModelElement))) : option (list (denoteModelClass type)) :=
-    denoteOutputList type (maybeResolveAll' tr sm name sp).
+    denoteOutputList type (maybeResolveAll tr sm name sp).
 
 End SemanticsModeling.
